typeclass 로부터 다른 typeclass 를 유도하는 방법은 참 많은데 말이야, 그걸 내가 정할 수는 없나?

doc/design/DotNet/Basic.lean
@@ -7,7 +7,8 @@ namespace DotNet
 structure TypeDef where
   name : String
   arity : Nat
-  deriving DecidableEq, BEq, Hashable
+  deriving DecidableEq, Hashable
+
 
 abbrev Pos := { x : Nat // 0 < x }
 
